theory/math/LogReal.dfy
@@ -10,24 +10,151 @@ module LogReal {
   import opened ExpReal
   import opened LemFunction
 
-  // log_b(x)
-  // We assert lem_log_NonNegative as post for convenience
-  ghost function {:axiom} log(b:real, x:real) : real
+  // There is exactly one y such that b^y = x
+  lemma {:axiom} lem_log_ExistsUnique(b:real, x:real)
     requires b > 1.0 && x > 0.0
-    ensures  b > 1.0 && x >= 1.0 ==> log(b, x) >= 0.0
+    ensures  exists y :: exp(b, y) == x
+    ensures  forall z1, z2 :: exp(b, z1) == x && exp(b, z2) == x ==> z1 == z2
+    // Proof.
+    // Existence by intermediate value theorem
+    // Uniquenes by injectivity implied by strictly increasing growth
 
-  // b > 1 ∧ x >= 1 ==> log_b(x) >= 0
-  lemma {:axiom} lem_log_NonNegative(b:real, x:real)
+  // log_b(x) = the unique y such that exp(b,y) = x
+  opaque ghost function log(b:real, x:real) : real
+    requires b > 1.0 && x > 0.0
+  {
+    lem_log_ExistsUnique(b, x);    
+    var y :| exp(b, y) == x;
+    y
+  }
+
+  /******************************************************************************
+    log_b(x) and b^x are inverses of each other for x ∈ (0,∞) and b > 1
+  ******************************************************************************/
+
+  // b^(log_b(x)) = x 
+  lemma lem_expLog_Inverse(b:real, x:real)
+    requires b > 1.0 && x > 0.0
+    ensures  exp(b, log(b, x)) == x
+  {
+    reveal log();
+  }
+
+  // log_b(b^x) = x 
+  lemma lem_logExp_Inverse(b:real, x:real)
+    requires b > 1.0
+    requires exp(b, x) > 0.0
+    ensures  log(b, exp(b, x)) == x 
+  {
+    // ensure the argument to log is in its domain:
+    assert exp(b, x) > 0.0 by { lem_exp_Positive(b, x); }
+    
+    // Invoke existence and uniqueness on exp(b, x)
+    ghost var v := exp(b, x);
+    assert && (exists u :: exp(b, u) == v) 
+           && (forall z1, z2 :: (exp(b, z1) == v) && (exp(b, z2) == v) ==> z1 == z2) 
+      by { lem_log_ExistsUnique(b, v); }
+    
+    // From the def. of choose, the chosen y satisfies the predicate: 
+    assert exp(b, log(b, exp(b, x))) == exp(b, x) by { reveal log(); }
+  }
+
+  // log and exp are mutual inverses on the domain x >= 1
+  // ∀ y : log_b(x) = y ⟺ b^y = x 
+  lemma lem_log_Inverse(b:real, x:real)
+    requires b > 1.0 && x >= 1.0 
+    ensures forall y :: (log(b, x) == y) <==> (exp(b, y) == x)
+  { 
+    forall y ensures (log(b, x) == y) <==> (exp(b, y) == x)
+    {
+      assert (log(b, x) == y) ==> (exp(b, y) == x) by {
+        if log(b, x) == y {
+          calc {
+               exp(b, y);
+            == exp(b, log(b, x));
+            == { lem_expLog_Inverse(b, x); }
+               x;      
+          }
+        }
+      }
+      assert (log(b, x) == y) <== (exp(b, y) == x) by {
+        if exp(b, y) == x {
+          calc {
+               log(b, x);
+            == log(b, exp(b, y));
+            == { lem_logExp_Inverse(b, y); }
+               y;      
+          }          
+        }
+      }
+    }
+  }
+
+  /******************************************************************************
+    Derived properties
+  ******************************************************************************/
+
+  // b > 1 ∧ x > 1 ⟹ log_b(x) > 0
+  lemma lem_log_Positive(b:real, x:real)
+    requires b > 1.0 && x > 1.0 
+    ensures  log(b, x) > 0.0 
+  {
+    var y := log(b, x);
+    assert exp(b, y) == x > 1.0 by { reveal log(); }       
+    assert exp(b, 0.0) == 1.0 by { lem_exp_Zero(b); }    
+    assert exp(b, 0.0) < exp(b, y); 
+    assert 0.0 < y by { lem_exp_StrictIncrIFF(b, y, 0.0); }    
+  }
+
+  lemma lem_log_PositiveAuto()
+    ensures forall b:real, x:real :: 
+            b > 1.0 && x > 1.0 ==> log(b, x) > 0.0
+  {
+    forall b:real, x:real | b > 1.0 && x > 1.0 
+      ensures log(b, x) > 0.0
+    {
+      lem_log_Positive(b, x);
+    }    
+  }
+
+  // b > 1 ∧ x >= 1 ⟹ log_b(x) >= 0
+  lemma lem_log_NonNegative(b:real, x:real)
     requires b > 1.0 && x >= 1.0 
     ensures  log(b, x) >= 0.0 
+  { 
+    if x == 1.0 {
+      assert log(b, 1.0) == 0.0 by { lem_log_One(b); }
+    } else {
+      lem_log_Positive(b, x);
+    }
+  }
 
-  // log_b(1) == 0
-  lemma {:axiom} lem_log_One(b:real)
+  lemma lem_log_NonNegativeAuto()
+    ensures forall b:real, x:real :: 
+            b > 1.0 && x >= 1.0 ==> log(b, x) >= 0.0
+  {
+    forall b:real, x:real | b > 1.0 && x >= 1.0 
+      ensures log(b, x) >= 0.0
+    {
+      lem_log_NonNegative(b, x);
+    }    
+  }
+
+  // log_b(1) = 0
+  lemma lem_log_One(b:real)
     requires b > 1.0
     ensures  log(b, 1.0) == 0.0
+  { 
+    calc {
+           log(b, 1.0) == 0.0;
+      <==> { lem_log_Inverse(b, 1.0); }
+           exp(b, 0.0) == 1.0;
+      <==> { lem_exp_Zero(b); }     
+           true;
+    }
+  }
 
-
-  // log_b(b) == 1.0
+  // log_b(b) = 1
   lemma lem_log_Base(b:real)
     requires b > 1.0
     ensures  log(b, b) == 1.0    
@@ -42,7 +169,7 @@ module LogReal {
     }
   }
   
-  // 1 < b <= x ==> log(b, x) >= 1
+  // 1 < b <= x ⟹ log(b, x) >= 1
   lemma lem_logGEQone(b:real, x:real)
     requires 1.0 < b <= x
     ensures  log(b, x) >= 1.0
@@ -56,36 +183,80 @@ module LogReal {
     }
   }  
 
+  // We can rewrite logarithms as a division of logarithms with the same base
+  // log_b(x) = log_c(x) / log_c(b)
+  lemma lem_log_ChangeOfBase(b:real, c:real, x:real)
+    requires b > 1.0 && c > 1.0 && x > 0.0
+    requires log(c, b) > 0.0
+    ensures  log(b, x) == log(c, x) / log(c, b)
+  {
+    // Let y = log(b, x)
+    var y := log(b, x);
+
+    // Rewrite the log in exp form
+    assert exp(b, y) == x by { lem_expLog_Inverse(b, x); }
+
+    // Express b in terms of base c
+    assert exp(c, log(c, b)) == b by { lem_expLog_Inverse(c, b); }
+
+    // Substitute b for exp(c, log(c, b)) in exp(b, y)
+    ghost var lg := log(c, b);
+    calc {
+         x;   
+      == exp(exp(c, lg), y);
+      == { lem_exp_Exp(c, lg, y); }
+         exp(c, lg * y);
+    }
+
+    // We want to relate with log_c(x). We also have
+    assert exp(c, log(c, x)) == x by { lem_expLog_Inverse(c, x); }
+
+    // Now we have c^(log_c(b)*y)=x and c^log_c(x)=x.
+    // By the uniqueness for base c: there is exactly one z with exp(c, z) == x
+    lem_log_ExistsUnique(c, x);
+    assert forall u, v :: exp(c, u) == x && exp(c, v) == x ==> u == v;
+
+    // So we have
+    assert log(c, x) == log(c, b) * y;
+
+    // Rearrange desired equality
+    assert y == log(b, x) == log(c, x) / log(c, b);
+  }
+
   /******************************************************************************
-    log_b(x) and b^x are inverses of each other for x ∈ (0,∞) and b > 1
-  ******************************************************************************/
-
-  // log_b(b^x) = x 
-  lemma {:axiom} lem_logExp_Inverse(b:real, x:real)
-    requires b > 1.0
-    requires exp(b, x) > 0.0
-    ensures  log(b, exp(b, x)) == x 
-
-  // b^(log_b(x)) = x 
-  lemma {:axiom} lem_expLog_Inverse(b:real, x:real)
-    requires b > 1.0 && x > 0.0
-    ensures  exp(b, log(b, x)) == x
-
-  /******************************************************************************
-    Order properties on the argument
+    Order properties on the positive argument
   ******************************************************************************/
   
   // For base b > 1, log_b(x) is strictly increasing on argument x ∈ (0,∞)
-  // b > 1 ∧ x,y > 0 ∧ x < y ==> log_b(x) < log_b(y)
-  lemma {:axiom} lem_log_StrictIncr(b:real, x:real, y:real)
-    requires b > 1.0 && x > 0.0 
+  // b > 1 ∧ x,y > 0 ∧ x < y ⟹ log_b(x) < log_b(y)  
+  lemma lem_log_StrictIncr(b:real, x:real, y:real)
+    requires b > 1.0 && x > 0.0 && y > 0.0 
     ensures  x < y ==> log(b, x) < log(b, y)
+  {
+    assert A: exp(b, log(b, x)) == x by { lem_expLog_Inverse(b, x); }
+    assert B: exp(b, log(b, y)) == y by { lem_expLog_Inverse(b, y); }
+    
+    if x < y {
+      assert exp(b, log(b, x)) < exp(b, log(b, y)) by { reveal A,B; }
+      if !(log(b, x) < log(b, y)) {
+        if log(b, x) == log(b, y) {
+          assert exp(b, log(b, x)) == exp(b, log(b, y));
+          assert false;
+        } else if log(b, x) > log(b, y) {
+          assert exp(b, log(b, x)) > exp(b, log(b, y)) 
+            by { lem_exp_StrictIncrIFF(b, log(b, x), log(b, y)); }
+          assert false; 
+        }
+      }
+      assert log(b, x) < log(b, y);
+    }
+  }
 
   lemma lem_log_StrictIncrAuto()
     ensures forall b:real, x:real, y:real :: 
-      b > 1.0 && x > 0.0 && x < y ==> log(b, x) < log(b, y)
+      b > 1.0 && x > 0.0 && y > 0.0 && x < y ==> log(b, x) < log(b, y)
   {
-    forall b:real, x:real, y:real | b > 1.0 && x > 0.0
+    forall b:real, x:real, y:real | b > 1.0 && x > 0.0 && y > 0.0
       ensures x < y ==> log(b, x) < log(b, y)
     {
       lem_log_StrictIncr(b, x, y);
@@ -93,7 +264,7 @@ module LogReal {
   }
 
   // Previous fact is reversible
-  // b > 1 ∧ x,y > 0 ∧ log_b(x) < log_b(y) ==> x < y
+  // b > 1 ∧ x,y > 0 ∧ log_b(x) < log_b(y) ⟹ x < y   
   lemma lem_log_StrictIncrRev(b:real, x:real, y:real)
     requires b > 1.0 && x > 0.0 && y > 0.0
     ensures  log(b, x) < log(b, y) ==> x < y
@@ -101,7 +272,7 @@ module LogReal {
     var log_b:real->real := (x => if x > 0.0 then log(b, x) else 0.0);
     assert forall x,y :: x > 0.0 && y > 0.0 ==> (x < y ==> log_b(x) < log_b(y))
       by { lem_log_StrictIncrAuto(); }
-    lem_fun_StrictIncrIMPinjectivePred(log_b, (x => x > 0.0));
+    lem_fun_StrictIncrIMPinjectiveRealPred(log_b, (x => x > 0.0));
     assert forall x,y :: x > 0.0 && y > 0.0 ==> (log_b(x) < log_b(y) ==> x < y);
     assert forall x :: x > 0.0 ==> log_b(x) == log(b, x);    
   }
@@ -118,7 +289,7 @@ module LogReal {
   }
 
   // Join previous facts into an equivalence
-  // b > 1 ∧ x,y > 0 ==> (x < y <==> log_b(x) < log_b(y))
+  // b > 1 ∧ x,y > 0 ⟹ (x < y ⟺ log_b(x) < log_b(y))
   lemma lem_log_StrictIncrIFF(b:real, x:real, y:real)
     requires b > 1.0 && x > 0.0 && y > 0.0
     ensures  x < y <==> (log(b, x) < log(b, y))
@@ -139,7 +310,7 @@ module LogReal {
   }
 
   // Weak version of lem_log_StrictIncrIFF
-  // b > 1 ∧ x,y > 0 ==> (x <= y <==> log_b(x) <= log_b(y))
+  // b > 1 ∧ x,y > 0 ⟹ (x <= y ⟺ log_b(x) <= log_b(y))
   lemma lem_log_MonoIncrIFF(b:real, x:real, y:real)
     requires b > 1.0 && x > 0.0 && y > 0.0
     ensures  x <= y <==> (log(b, x) <= log(b, y))
@@ -163,10 +334,37 @@ module LogReal {
   ******************************************************************************/
 
   // When x ∈ (1,∞), log_b(x) is strictly decreasing on b
-  // b1, b2 > 1 ∧ x > 1 ∧ b1 < b2 ==> log_b1(x) > log_b2(x)
+  // b1,b2 > 1 ∧ x > 1 ∧ b1 < b2 ⟹ log_b1(x) > log_b2(x)
   lemma {:axiom} lem_log_BaseStrictDecr(b1:real, b2:real, x:real)
     requires b1 > 1.0 && b2 > 1.0 && x > 1.0
     ensures  b1 < b2 ==> log(b1, x) > log(b2, x)     
+  {
+    // First let's define locally the log operation on fixed base 2
+    ghost var log2:real-->real := x requires x > 0.0 => log(2.0, x);
+    // Some facts for log2
+    assert A : log2(x) > 0.0 
+      by { lem_log_Positive(2.0, x); }
+    assert B : log2(b1) > 0.0 
+      by { lem_log_Positive(2.0, b1); }     
+    assert C : b1 < b2 ==> log2(b1) < log2(b2)
+      by { lem_log_StrictIncr(2.0, b1, b2); }
+
+    // Now, for the proof
+    if b1 < b2 {
+      assert 0.0 < log2(x) by { reveal A; }
+      assert 0.0 < log2(b1) < log2(b2) by { reveal B, C; }
+      calc {
+             log2(b1) < log2(b2);
+        <==> log2(x) * log2(b1) < log2(x) * log2(b2);
+        <==> log2(x) / log2(b2) < log2(x) / log2(b1);
+        <==> log2(x) / log2(b1) > log2(x) / log2(b2);
+        <==> { lem_log_ChangeOfBase(b1, 2.0, x);  }
+             log(b1, x) > log2(x) / log2(b2);
+        <==> { lem_log_ChangeOfBase(b2, 2.0, x);  }
+             log(b1, x) > log(b2, x);             
+      } 
+    }
+  }
 
   lemma lem_log_BaseStrictDecrAuto()
     ensures forall b1:real, b2:real, x:real :: 
@@ -180,7 +378,7 @@ module LogReal {
   }
 
   // Previous fact is reversible
-  // b1, b2 > 1 ∧ x > 1 ∧ log_b1(x) > log_b2(x) ==> b1 < b2
+  // b1,b2 > 1 ∧ x > 1 ∧ log_b1(x) > log_b2(x) ⟹ b1 < b2
   lemma lem_log_BaseStrictDecrRev(b1:real, b2:real, x:real)
     requires b1 > 1.0 && b2 > 1.0 && x > 1.0
     ensures  log(b1, x) > log(b2, x) ==> b1 < b2
@@ -188,7 +386,7 @@ module LogReal {
     var log_x:real->real := (b => if b > 1.0 then log(b, x) else 0.0);
     assert forall b1,b2 :: b1 > 1.0 && b2 > 1.0 ==> (b1 < b2 ==> log_x(b1) > log_x(b2))
       by { lem_log_BaseStrictDecrAuto(); }
-    lem_fun_StrictDecrIMPinjectivePred(log_x, (b => b > 1.0));
+    lem_fun_StrictDecrIMPinjectiveRealPred(log_x, (b => b > 1.0));
     assert forall b1,b2 :: b1 > 1.0 && b2 > 1.0 ==> (log_x(b1) > log_x(b2) ==> b1 < b2);
     assert forall b :: b > 1.0 ==> log_x(b) == log(b, x);       
   } 
@@ -205,7 +403,7 @@ module LogReal {
   }
 
   // Join previous facts into an equivalence
-  // b1, b2 > 1 ∧ x > 1 ==> (b1 < b2 <==> log_b1(x) > log_b2(x))
+  // b1,b2 > 1 ∧ x > 1 ⟹ (b1 < b2 ⟺ log_b1(x) > log_b2(x))
   lemma lem_log_BaseStrictDecrIFF(b1:real, b2:real, x:real)
     requires b1 > 1.0 && b2 > 1.0 && x > 1.0
     ensures  b1 < b2 <==> log(b1, x) > log(b2, x)
@@ -226,7 +424,7 @@ module LogReal {
   }
 
   // Weak version of lem_log_BaseStrictDecrIFF
-  // b1, b2 > 1 ∧ x > 1 ==> (b1 <= b2 <==> log_b1(x) >= log_b2(x))
+  // b1,b2 > 1 ∧ x > 1 ⟹ (b1 <= b2 ⟺ log_b1(x) >= log_b2(x))
   lemma lem_log_BaseMonoDecrIFF(b1:real, b2:real, x:real)
     requires b1 > 1.0 && b2 > 1.0 && x > 1.0
     ensures  b1 <= b2 <==> log(b1, x) >= log(b2, x)  
@@ -246,7 +444,7 @@ module LogReal {
   }
 
   // Weak version of lem_log_BaseStrictDecr, but also holds when x=1
-  // b1, b2 > 1 ∧ x >= 1 ∧ b1 <= b2 ==> log_b1(x) >= log_b2(x)
+  // b1,b2 > 1 ∧ x >= 1 ∧ b1 <= b2 ⟹ log_b1(x) >= log_b2(x)
   lemma lem_log_BaseMonoDecr(b1:real, b2:real, x:real)
     requires b1 > 1.0 && b2 > 1.0 && x >= 1.0
     ensures  b1 <= b2 ==> log(b1, x) >= log(b2, x)  
@@ -268,22 +466,6 @@ module LogReal {
     {
       lem_log_BaseMonoDecr(b1, b2, x);
     }       
-  }
-
-  /******************************************************************************
-    Universal closures of lemmas
-  ******************************************************************************/
-
-  // b > 1 /\ x >= 1 ==> log_b(x) >= 0
-  lemma lem_log_NonNegativeAuto()
-    ensures  forall b:real, x:real :: 
-             b > 1.0 && x >= 1.0 ==> log(b, x) >= 0.0
-  {
-    forall b:real, x:real | b > 1.0 && x >= 1.0 
-      ensures log(b, x) >= 0.0
-    {
-      lem_log_NonNegative(b, x);
-    }    
   }
 
 }
