caseStudy/ADT/List/List.dfy
@@ -76,8 +76,8 @@ module List {
       // Post:
       ensures  Valid()
       ensures  Size() == old(Size()) - 1
-      ensures  forall j :: 0 <= j < k      ==> Get(j).0 == old(Get(j).0)
-      ensures  forall j :: k <= j < Size() ==> Get(j).0 == old(Get(j+1).0)
+      ensures  forall j :: 0 <= j < k      ==> Get(j).0 == old(Get(j).0)    // [0, k) is unchanged
+      ensures  forall j :: k <= j < Size() ==> Get(j).0 == old(Get(j+1).0)  // (k, old(Size())) is left shifted  
 
   }  
 
