theory/math/ExpNat.dfy
@@ -1,9 +1,14 @@
+include "./LemFunction.dfy"
+//include "./Order.dfy"
 
 /******************************************************************************
   Exponentiation over non-negative integers
 ******************************************************************************/
 
 module ExpNat {
+
+  import opened LemFunction
+  //import opened Order
 
   // b^e
   opaque ghost function exp(b:nat, e:nat) : nat
@@ -12,30 +17,7 @@ module ExpNat {
     if e == 0 then 1 else b*exp(b, e-1)
   }
 
-  // b >= 1 /\ n <= m ==> b^n <= b^m
-  lemma lem_exp_MonoIncr(b:nat, n:nat, m:nat)
-    requires b >= 1
-    ensures  n <= m ==> exp(b, n) <= exp(b, m)
-    decreases n, m
-  { 
-    reveal exp();
-    if n != 0 && m != 0 {  
-      lem_exp_MonoIncr(b, n-1, m-1); 
-    }
-  }
-
-  // n <= m ==> n^e <= m^e
-  lemma {:axiom} lem_exp_BaseMonoIncr(e:nat, n:nat, m:nat)
-    ensures n <= m ==> exp(n, e) <= exp(m, e)
-    decreases n, m
-  // {   // TODO
-  //   reveal exp();
-  //   if n != 0 && m != 0 {  
-  //     lem_exp_BaseMonoIncr(e, n-1, m-1); 
-  //   }
-  // }  
-
-  // b>0 ==> b^e > 0
+  // b > 0 ⟹ b^e > 0
   lemma lem_exp_Positive(b:nat, e:nat)
     requires b > 0
     ensures exp(b,e) > 0
@@ -63,33 +45,199 @@ module ExpNat {
   }
   
   /******************************************************************************
-    Relate to dafny primitive powers
+    Relate exp(x,0), exp(x,1), exp(x,2), etc. to Dafny primitive powers
   ******************************************************************************/
 
-  // n^1 == n
+  // n^0 = 1
+  lemma lem_exp_Pow0(n:nat)
+    ensures exp(n,0) == 1
+  { 
+    reveal exp;
+  }
+
+  lemma lem_exp_Pow0Auto()
+    ensures forall n:nat :: exp(n,0) == 1  
+  { 
+    forall n:nat ensures exp(n,0) == 1 {
+      lem_exp_Pow0(n);
+    }
+  }
+
+  // n^1 = n
   lemma lem_exp_Pow1(n:nat)
     ensures exp(n,1) == n
-  { reveal exp; }
+  { 
+    reveal exp;
+  }
 
-  // n^2 == n*n
+  lemma lem_exp_Pow1Auto()
+    ensures forall n:nat :: exp(n,1) == n  
+  { 
+    forall n:nat ensures exp(n,1) == n {
+      lem_exp_Pow1(n);
+    }
+  }
+
+  // n^2 = n*n
   lemma lem_exp_Pow2(n:nat)
     ensures exp(n,2) == n*n
-  { reveal exp; }  
+  { 
+    reveal exp; 
+  }  
 
-  // n^3 == n*n*n
+  lemma lem_exp_Pow2Auto()
+    ensures forall n:nat :: exp(n,2) == n*n  
+  {
+    forall n:nat ensures exp(n,2) == n*n {
+      lem_exp_Pow2(n);
+    }
+  } 
+
+  // n^3 = n*n*n
   lemma lem_exp_Pow3(n:nat)
     ensures exp(n,3) == n*n*n  
   { reveal exp; }  
+
+  lemma lem_exp_Pow3Auto()
+    ensures forall n:nat :: exp(n,3) == n*n*n 
+  {
+    forall n:nat ensures exp(n,3) == n*n*n {
+      lem_exp_Pow3(n);
+    }
+  } 
+
+  /******************************************************************************
+    Order properties on the exponent with base >= 1 (or > 1)
+  ******************************************************************************/
+
+  // b > 1 ∧ n < m ⟹ b^n < b^m
+  lemma lem_exp_StrictIncr(b:nat, n:nat, m:nat)
+    requires b > 1
+    ensures  n < m ==> exp(b, n) < exp(b, m)
+    decreases n, m
+  { 
+    reveal exp();
+    if n != 0 && m != 0 {  
+      lem_exp_StrictIncr(b, n-1, m-1); 
+    }
+  }
+
+  lemma lem_exp_StrictIncrAuto()
+    ensures forall b:nat, n:nat, m:nat :: 
+      b > 1 && n < m ==> exp(b, n) < exp(b, m)
+  {
+    forall b:nat, n:nat, m:nat | b > 1
+      ensures n < m ==> exp(b, n) < exp(b, m)
+    {
+      lem_exp_StrictIncr(b, n, m);
+    }       
+  }
+
+  // Previous fact is reversible
+  // b > 1 ∧ b^n < b^m ⟹ n < m
+  lemma lem_exp_StrictIncrRev(b:nat, n:nat, m:nat)
+    requires b > 1
+    ensures  exp(b, n) < exp(b, m) ==> n < m
+  { 
+    var exp_b:nat->nat := x => exp(b, x);
+    assert forall x,y :: x < y ==> exp_b(x) < exp_b(y)
+      by { lem_exp_StrictIncrAuto(); }
+    lem_fun_StrictIncrIMPinjectiveNat(exp_b);
+    assert forall x,y :: exp_b(x) < exp_b(y) ==> x < y;
+    assert forall x :: exp_b(x) == exp(b, x);
+  }
+
+  lemma lem_exp_StrictIncrRevAuto()
+    ensures forall b:nat, n:nat, m:nat :: 
+      b > 1 && exp(b, n) < exp(b, m) ==> n < m
+  {
+    forall b:nat, n:nat, m:nat | b > 1
+      ensures exp(b, n) < exp(b, m) ==> n < m
+    {
+      lem_exp_StrictIncrRev(b, n, m);
+    }       
+  }  
+
+  // Join previous facts into an equivalence
+  // b > 1 ⟹ (x < y ⟺ b^x < b^y)
+  lemma lem_exp_StrictIncrIFF(b:nat, n:nat, m:nat)
+    requires b > 1
+    ensures  n < m <==> exp(b, n) < exp(b, m)
+  { 
+    lem_exp_StrictIncr(b,n,m);
+    lem_exp_StrictIncrRev(b,n,m);
+  }
+
+  lemma lem_exp_StrictIncrIFFAuto()
+    ensures forall b:nat, n:nat, m:nat :: 
+      b > 1 ==> (n < m <==> exp(b, n) < exp(b, m))
+  {
+    forall b:nat, n:nat, m:nat | b > 1
+      ensures n < m <==> exp(b, n) < exp(b, m)
+    {
+      lem_exp_StrictIncrIFF(b, n, m);
+    }       
+  }    
+
+  // Weak version of lem_exp_StrictIncrIFF
+  // b > 1 ⟹ (x <= y ⟺ b^x <= b^y)
+  lemma lem_exp_MonoIncrIFF(b:nat, n:nat, m:nat)
+    requires b > 1
+    ensures  n <= m <==> exp(b, n) <= exp(b, m)
+  {
+    lem_exp_StrictIncrIFFAuto();
+  }
+
+  lemma lem_exp_MonoIncrIFFAuto()
+    ensures forall b:nat, n:nat, m:nat :: 
+      b > 1 ==> (n <= m <==> exp(b, n) <= exp(b, m))
+  {
+    forall b:nat, n:nat, m:nat | b > 1
+      ensures n <= m <==> exp(b, n) <= exp(b, m)
+    {
+      lem_exp_MonoIncrIFF(b, n, m);
+    }       
+  }  
+
+  // Weak version of lem_exp_StrictIncr, but also holds when b=1
+  // b >= 1 ∧ n <= m ⟹ b^n <= b^m
+  lemma lem_exp_MonoIncr(b:nat, n:nat, m:nat)
+    requires b >= 1
+    ensures  n <= m ==> exp(b, n) <= exp(b, m)
+    decreases n, m
+  { 
+    if b == 1 {
+      reveal exp();
+    } else if b > 1 {
+      lem_exp_StrictIncr(b, n, m);
+    }    
+  }
+
+  /******************************************************************************
+    Order properties on the base
+  ******************************************************************************/
+  
+  
+  // n <= m ⟹ n^e <= m^e
+  lemma {:axiom} lem_exp_BaseMonoIncr(e:nat, n:nat, m:nat)
+    ensures n <= m ==> exp(n, e) <= exp(m, e)
+    decreases n, m
+  // {   // TODO
+  //   reveal exp();
+  //   if n != 0 && m != 0 {  
+  //     lem_exp_BaseMonoIncr(e, n-1, m-1); 
+  //   }
+  // }  
 
   /******************************************************************************
     Binomial expansion
   ******************************************************************************/
 
-  // (n+1)^2 == n*n + 2*n + 1
+  // (n+1)^2 = n*n + 2*n + 1
   lemma {:axiom} lem_exp_binomial(n:nat)
     ensures exp(n+1,2) == n*n + 2*n + 1
 
-  // n^2 == (n-1)*2 + 2*(n-1) + 1
+  // n^2 = (n-1)*2 + 2*(n-1) + 1
   lemma {:axiom} lem_exp_binomial2(n:nat)
     requires n > 0
     ensures exp(n,2) == exp(n-1,2) + 2*(n-1) + 1 
@@ -113,33 +261,5 @@ module ExpNat {
   {
     reveal exp();
   }  
-
-  /******************************************************************************
-    Universal clausures of lemmas
-  ******************************************************************************/
-
-  lemma lem_exp_Pow1Auto()
-    ensures forall n:nat :: exp(n,1) == n  
-  { 
-    forall n:nat ensures exp(n,1) == n {
-      lem_exp_Pow1(n);
-    }
-  }
-
-  lemma lem_exp_Pow2Auto()
-    ensures forall n:nat :: exp(n,2) == n*n  
-  {
-    forall n:nat ensures exp(n,2) == n*n {
-      lem_exp_Pow2(n);
-    }
-  }  
-
-  lemma lem_exp_Pow3Auto()
-    ensures forall n:nat :: exp(n,3) == n*n*n 
-  {
-    forall n:nat ensures exp(n,3) == n*n*n {
-      lem_exp_Pow3(n);
-    }
-  }   
 
 }
