theory/math/ExpR0.dfy
@@ -1,5 +1,6 @@
 include "./ExpNat.dfy"
 include "./LemFunction.dfy"
+include "./LemReal.dfy"
 include "./TypeR0.dfy"
 
 /******************************************************************************
@@ -15,15 +16,21 @@ module ExpR0 {
 
   import N = ExpNat
   import opened LemFunction
+  import opened LemReal
   import opened TypeR0
 
   // x^y
   ghost function {:axiom} exp(x:R0, y:R0) : R0
 
-  // x > 0 ==> x^y > 0
+  // x > 0 ⟹ x^y > 0
   lemma {:axiom} lem_exp_Positive(x:R0, y:R0)
     requires x > 0.0
     ensures  exp(x, y) > 0.0         
+
+  // x > 1 ∧ y > 0 ⟹ x^y > 1
+  lemma {:axiom} lem_exp_GTone(x:R0, y:R0)
+    requires x > 1.0 && y > 0.0
+    ensures  exp(x, y) > 1.0     
 
   // x^0 = 1
   lemma {:axiom} lem_exp_Zero(x:R0)
@@ -33,7 +40,7 @@ module ExpR0 {
   lemma {:axiom} lem_exp_One(x:R0)
     ensures  exp(x, 1.0) == x
 
-  // y > 0 ==> 0^y = 0
+  // y > 0 ⟹ 0^y = 0
   lemma {:axiom} lem_exp_BaseZero(y:R0)
     requires y > 0.0
     ensures  exp(0.0, y) == 0.0     
@@ -50,21 +57,116 @@ module ExpR0 {
   lemma {:axiom} lem_exp_Exp(x:R0, y:R0, z:R0)
     ensures  exp(exp(x, y), z) == exp(x, y*z) 
 
-  lemma lem_exp_ExpAuto()
+  // The only other axiom we take is lem_exp_BaseStrictIncr, see below in the list
+  // of order properties on the base
+
+  /******************************************************************************
+    Universal closures of the axioms
+  ******************************************************************************/
+
+  lemma lem_exp_PositiveAuto()
+    ensures forall x:real, y:real ::  
+            x > 0.0 && y >= 0.0 ==> exp(x, y) > 0.0
+  {
+     forall x:real, y:real | x > 0.0 && y >= 0.0
+      ensures exp(x, y) > 0.0
+    {
+      lem_exp_Positive(x, y);
+    }
+  }  
+
+  lemma lem_exp_GToneAuto()
+    ensures forall x:R0, y:R0 ::  
+            x > 1.0 && y > 0.0 ==> exp(x, y) > 1.0
+  {
+     forall x:R0, y:R0 | x > 1.0 && y > 0.0
+      ensures exp(x, y) > 1.0
+    {
+      lem_exp_GTone(x, y);
+    }
+  } 
+
+  lemma lem_exp_ZeroAuto()
+    ensures forall x:R0 :: x > 0.0 ==> exp(x, 0.0) == 1.0 
+  {
+    forall x:R0 | x > 0.0
+      ensures exp(x, 0.0) == 1.0 
+    {
+      lem_exp_Zero(x);
+    }
+  }
+
+  lemma lem_exp_OneAuto()
+    ensures forall x:R0 :: x > 0.0 ==> exp(x, 1.0) == x 
+  {
+    forall x:R0 | x > 0.0
+      ensures exp(x, 1.0) == x 
+    {
+      lem_exp_One(x);
+    }    
+  }
+
+  lemma lem_exp_BaseZeroAuto()
+    ensures forall y:R0 :: y > 0.0 ==> exp(0.0, y) == 0.0 
+  {
+    forall y:R0 | y > 0.0
+      ensures exp(0.0, y) == 0.0 
+    {
+      lem_exp_BaseZero(y);
+    }
+  }
+
+  lemma lem_exp_BaseOneAuto()
+    ensures forall y:R0 :: exp(1.0, y) == 1.0 
+  {
+    forall y:R0
+      ensures exp(1.0, y) == 1.0 
+    {
+      lem_exp_BaseOne(y);
+    }
+  }
+
+  lemma lem_exp_ProductAuto()
     ensures forall x:R0, y:R0, z:R0 :: 
-      exp(exp(x, y), z) == exp(x, y*z) 
+      exp(x, y+z) == exp(x, y)*exp(x, z)
   {
     forall x:R0, y:R0, z:R0
+      ensures exp(x, y+z) == exp(x, y)*exp(x, z)
+    {
+      lem_exp_Product(x, y, z);
+    }   
+  }
+
+  lemma lem_exp_ExpAuto()
+    ensures forall x:R0, y:R0, z:R0 :: 
+            x >= 0.0 ==> exp(exp(x, y), z) == exp(x, y*z) 
+  {
+    forall x:R0, y:R0, z:R0 | x >= 0.0
       ensures exp(exp(x, y), z) == exp(x, y*z) 
     {
       lem_exp_Exp(x, y, z);
     }   
   }
 
-  // x >= 1 ==> x^y >= 1
+  /******************************************************************************
+    Derived properties
+  ******************************************************************************/
+
+  // x >= 1 ⟹ x^y >= 1
   lemma {:axiom} lem_exp_GEQone(x:R0, y:R0)
     requires x >= 1.0
     ensures  exp(x, y) >= 1.0  
+
+  lemma lem_exp_GEQoneAuto()
+    ensures forall x:real, y:real :: 
+      x >= 1.0 && y >= 0.0 ==> exp(x, y) >= 1.0  
+  {
+    forall x:real, y:real | x >= 1.0 && y >= 0.0
+      ensures exp(x, y) >= 1.0  
+    {
+      lem_exp_GEQone(x, y);
+    }
+  }
 
   // x*(x^y) = x^(y+1)
   lemma lem_exp_Def(x:R0, y:R0)
@@ -77,18 +179,53 @@ module ExpR0 {
       == { lem_exp_Product(x, 1.0, y); }
           exp(x, y + 1.0);
     } 
-
   } 
 
+  lemma lem_exp_DefAuto()
+    ensures forall x:R0, y:R0 :: 
+      x*exp(x, y) == exp(x, y + 1.0)
+  {
+    forall x:R0, y:R0
+      ensures x*exp(x, y) == exp(x, y + 1.0)
+    {
+      lem_exp_Def(x, y);
+    }
+  }
+
   /******************************************************************************
-    Relate to dafny primitive powers
+    Relate exp(x,0), exp(x,1), exp(x,2), etc. to Dafny primitive powers
   ******************************************************************************/
+
+  // x^0 = 1
+  lemma lem_exp_Pow0(x:R0) 
+    ensures exp(x, 0.0) == 1.0
+  { 
+    lem_exp_Zero(x);
+  }
+
+  lemma lem_exp_Pow0Auto()
+    ensures forall x:R0 :: exp(x, 0.0) == 1.0
+  {
+    forall x:R0 ensures exp(x, 0.0) == 1.0
+    {
+      lem_exp_Pow0(x);
+    }
+  }
 
   // x^1 = x
   lemma lem_exp_Pow1(x:R0) 
     ensures exp(x, 1.0) == x
   { 
     lem_exp_One(x);
+  }
+
+  lemma lem_exp_Pow1Auto()
+    ensures forall x:R0 :: exp(x, 1.0) == x
+  {
+    forall x:R0 ensures exp(x, 1.0) == x
+    {
+      lem_exp_Pow1(x);
+    }
   }
 
   // x^2 = x*x
@@ -108,6 +245,15 @@ module ExpR0 {
     }
   } 
 
+  lemma lem_exp_Pow2Auto()
+    ensures forall x:R0 :: exp(x, 2.0) == x*x
+  {
+    forall x:R0 ensures exp(x, 2.0) == x*x
+    {
+      lem_exp_Pow2(x);
+    }
+  }
+
   // x^3 = x*x*x
   lemma lem_exp_Pow3(x:R0) 
     ensures exp(x, 3.0) == x*x*x
@@ -123,6 +269,15 @@ module ExpR0 {
       == x*x*x; 
     } 
   }    
+
+  lemma lem_exp_Pow3Auto()
+    ensures forall x:R0 :: exp(x, 3.0) == x*x*x
+  {
+    forall x:R0 ensures exp(x, 3.0) == x*x*x
+    {
+      lem_exp_Pow3(x);
+    }
+  }
 
   /******************************************************************************
     Extend exp for negative exponents
@@ -141,10 +296,25 @@ module ExpR0 {
   ******************************************************************************/
 
   // Strict increasing
-  // b > 1 ∧ x < y ==> b^x < b^y
+  // b > 1 ∧ x < y ⟹ b^x < b^y
   lemma {:axiom} lem_exp_StrictIncr(b:R0, x:R0, y:R0)
     requires b > 1.0
     ensures  x < y ==> exp(b, x) < exp(b, y)
+  {
+    if x < y {
+      var d :| d > 0.0 && y == x + d
+        by { lem_real_PosDifference(x, y); } 
+      assert A: exp(b, x) > 0.0 by { lem_exp_Positive(b, x);}
+      calc {
+           exp(b, y);
+        == { lem_exp_Product(b, x, d); }
+           exp(b, x) * exp(b, d);
+        >  { assert d > 0.0; lem_exp_GTone(b, d); reveal A; }
+           exp(b, x) * 1.0;
+        == exp(b, x);       
+      }
+    }
+  }
 
   lemma lem_exp_StrictIncrAuto()
     ensures forall b:R0, x:R0, y:R0 :: 
@@ -158,7 +328,7 @@ module ExpR0 {
   }
 
   // Previous fact is reversible
-  // b > 1 ∧ b^x < b^y ==> x < y
+  // b > 1 ∧ b^x < b^y ⟹ x < y
   lemma lem_exp_StrictIncrRev(b:R0, x:R0, y:R0)
     requires b > 1.0
     ensures  exp(b, x) < exp(b, y) ==> x < y
@@ -183,7 +353,7 @@ module ExpR0 {
   }  
 
   // Join previous facts into an equivalence
-  // b > 1 ==> x < y <==> b^x < b^y
+  // b > 1 ⟹ (x < y ⟺ b^x < b^y)
   lemma lem_exp_StrictIncrIFF(b:R0, x:R0, y:R0)
     requires b > 1.0
     ensures  x < y <==> exp(b, x) < exp(b, y)
@@ -204,7 +374,7 @@ module ExpR0 {
   }    
 
   // Weak version of lem_exp_StrictIncrIFF
-  // b > 1 ==> (x <= y <==> b^x <= b^y)
+  // b > 1 ⟹ (x <= y ⟺ b^x <= b^y)
   lemma lem_exp_MonoIncrIFF(b:R0, x:R0, y:R0)
     requires b > 1.0
     ensures  x <= y <==> exp(b, x) <= exp(b, y)
@@ -224,7 +394,7 @@ module ExpR0 {
   }  
 
   // Weak version of lem_exp_StrictIncr, but also holds when x=1
-  // b >= 1 ∧ x <= y ==> b^x <= b^y
+  // b >= 1 ∧ x <= y ⟹ b^x <= b^y
   lemma lem_exp_MonoIncr(b:R0, x:R0, y:R0)
     requires b >= 1.0
     ensures  x <= y ==> exp(b, x) <= exp(b, y)
@@ -242,7 +412,7 @@ module ExpR0 {
   ******************************************************************************/
 
   // Strictly decreasing
-  // 0 < b < 1 ∧ x < y ==> b^x > b^y   
+  // 0 < b < 1 ∧ x < y ⟹ b^x > b^y   
   lemma {:axiom} lem_exp_StrictDecr(b:R0, x:R0, y:R0)
     requires 0.0 < b < 1.0
     ensures x < y ==> exp(b, x) > exp(b, y) 
@@ -259,7 +429,7 @@ module ExpR0 {
   }
 
   // Previous fact is reversible
-  // 0 < b < 1 ∧ b^x > b^y ==> x < y
+  // 0 < b < 1 ∧ b^x > b^y ⟹ x < y
   lemma lem_exp_StrictDecrRev(b:R0, x:R0, y:R0)
     requires 0.0 < b < 1.0
     ensures exp(b, x) > exp(b, y) ==> x < y
@@ -284,7 +454,7 @@ module ExpR0 {
   }  
 
   // Join previous facts into an equivalence
-  // 0 < b < 1 ==> (x < y <==> b^x > b^y)  
+  // 0 < b < 1 ⟹ (x < y ⟺ b^x > b^y)  
   lemma lem_exp_StrictDecrIFF(b:R0, x:R0, y:R0)
     requires 0.0 < b < 1.0
     ensures x < y <==> exp(b, x) > exp(b, y)
@@ -305,7 +475,7 @@ module ExpR0 {
   }  
 
   // Weak version of lem_exp_StrictDecrIFF
-  // 0 < b < 1 ==> (x <= y <==> b^x >= b^y) 
+  // 0 < b < 1 ⟹ (x <= y ⟺ b^x >= b^y) 
   lemma lem_exp_AntiMonoIncrIFF(b:R0, x:R0, y:R0)
     requires 0.0 < b < 1.0
     ensures x <= y <==> exp(b, x) >= exp(b, y)
@@ -325,11 +495,11 @@ module ExpR0 {
   }  
 
   /******************************************************************************
-    Order properties on the base for exponent >= 0 (or e > 0)
+    Order properties on the base for exponent >= 0 (or > 0)
   ******************************************************************************/
 
   // Strictly increasing
-  // e > 0 ∧ x,y >= 0 ∧ x < y ==> x^e < y^e
+  // e > 0 ∧ x,y >= 0 ∧ x < y ⟹ x^e < y^e
   lemma {:axiom} lem_exp_BaseStrictIncr(e:real, x:real, y:real)
     requires e > 0.0 && x >= 0.0 && y >= 0.0
     ensures  x < y ==> exp(x, e) < exp(y, e)    
@@ -346,7 +516,7 @@ module ExpR0 {
   }
 
   // Previous fact is reversible
-  // e > 0 ∧ x,y >= 0 ∧ x^e < y^e ==> x < y
+  // e > 0 ∧ x,y >= 0 ∧ x^e < y^e ⟹ x < y
   lemma lem_exp_BaseStrictIncrRev(e:real, x:real, y:real)
     requires e > 0.0 && x >= 0.0 && y >= 0.0
     ensures  exp(x, e) < exp(y, e) ==> x < y
@@ -371,7 +541,7 @@ module ExpR0 {
   }
 
   // Join previous facts into an equivalence
-  // e > 0 ∧ x,y >= 0 ==> (x < y <==> x^e < y^e)
+  // e > 0 ∧ x,y >= 0 ⟹ (x < y ⟺ x^e < y^e)
   lemma lem_exp_BaseStrictIncrIFF(e:real, x:real, y:real) 
     requires e > 0.0 && x >= 0.0 && y >= 0.0
     ensures  x < y <==> exp(x, e) < exp(y, e)
@@ -392,7 +562,7 @@ module ExpR0 {
   }
 
   // Weak version of lem_exp_BaseStrictIncrIFF
-  // e > 0 ∧ x,y >= 0 ==> (x <= y <==> x^e <= y^e)
+  // e > 0 ∧ x,y >= 0 ⟹ (x <= y ⟺ x^e <= y^e)
   lemma lem_exp_BaseMonoIncrIFF(e:real, x:real, y:real) 
     requires e > 0.0 && x >= 0.0 && y >= 0.0
     ensures  x <= y <==> exp(x, e) <= exp(y, e)
@@ -413,7 +583,7 @@ module ExpR0 {
 
   // A weak version of lem_exp_BaseStrictIncr, also holds when x=0
   // but is restricted to x,y > 0
-  // e >= 0 ∧ x,y > 0 ∧ x <= y ==> x^e <= y^e
+  // e >= 0 ∧ x,y > 0 ∧ x <= y ⟹ x^e <= y^e
   lemma lem_exp_BaseMonoIncr(e:real, x:real, y:real)
     requires e >= 0.0 && x > 0.0 && y > 0.0
     ensures  x <= y ==> exp(x, e) <= exp(y, e)
@@ -508,7 +678,7 @@ module ExpR0 {
     N.lem_exp2_FirstValues();
   }    
 
-  // x < y ==> 2^x < 2^y
+  // x < y ⟹ 2^x < 2^y
   lemma lem_exp2_StrictIncr(x:R0, y:R0)
     ensures x < y ==> exp2(x) < exp2(y)  
   {
@@ -516,7 +686,7 @@ module ExpR0 {
     lem_exp_StrictIncr(2.0, x, y);
   }
 
-  // 2^x < 2^y ==> x < y
+  // 2^x < 2^y ⟹ x < y
   lemma lem_exp2_StrictIncrRev(x:R0, y:R0)
     ensures exp2(x) < exp2(y) ==> x < y
   {
@@ -524,7 +694,7 @@ module ExpR0 {
     lem_exp_StrictIncrRev(2.0, x, y);
   }  
 
-  // x < y <==> 2^x < 2^y 
+  // x < y ⟺ 2^x < 2^y 
   lemma lem_exp2_StrictIncrIFF(x:R0, y:R0)
     ensures x < y <==> exp2(x) < exp2(y) 
   {
@@ -532,79 +702,11 @@ module ExpR0 {
     lem_exp_StrictIncrIFF(2.0, x, y);
   }    
 
-  // x <= y ==> 2^x <= 2^y
+  // x <= y ⟹ 2^x <= 2^y
   lemma lem_exp2_MonoIncr(x:R0, y:R0)
     ensures x <= y ==> exp2(x) <= exp2(y)  
   {
     lem_exp2_StrictIncr(x, y);
-  }
-
-  /******************************************************************************
-    Universal closures of lemmas
-  ******************************************************************************/
-
-  // x > 0 ∧ y >= 0 ==> x^y > 0
-  lemma lem_exp_PositiveAuto()
-    ensures forall x:real, y:real ::  
-            x > 0.0 && y >= 0.0 ==> exp(x, y) > 0.0
-  {
-     forall x:real, y:real | x > 0.0 && y >= 0.0
-      ensures exp(x, y) > 0.0
-    {
-      lem_exp_Positive(x, y);
-    }
-  }  
-
-  lemma lem_exp_ZeroAuto()
-    ensures forall x:R0 :: x > 0.0 ==> exp(x, 0.0) == 1.0 
-  {
-    forall x:R0 | x > 0.0
-      ensures exp(x, 0.0) == 1.0 
-    {
-      lem_exp_Zero(x);
-    }
-  }
-
-  lemma lem_exp_OneAuto()
-    ensures forall x:R0 :: x > 0.0 ==> exp(x, 1.0) == x 
-  {
-    forall x:R0 | x > 0.0
-      ensures exp(x, 1.0) == x 
-    {
-      lem_exp_One(x);
-    }    
-  }
-
-  lemma lem_exp_ProductAuto()
-    ensures forall x:R0, y:R0, z:R0 :: 
-      exp(x, y+z) == exp(x, y)*exp(x, z)
-  {
-    forall x:R0, y:R0, z:R0
-      ensures exp(x, y+z) == exp(x, y)*exp(x, z)
-    {
-      lem_exp_Product(x, y, z);
-    }   
-  }
-
-  lemma lem_exp_Pow2Auto()
-    ensures forall x:R0 :: exp(x, 2.0) == x*x
-  {
-    forall x:R0
-      ensures exp(x, 2.0) == x*x
-    {
-      lem_exp_Pow2(x);
-    }
-  }
-
-  lemma lem_exp_DefAuto()
-    ensures forall x:R0, y:R0 :: 
-      x*exp(x, y) == exp(x, y + 1.0)
-  {
-    forall x:R0, y:R0
-      ensures x*exp(x, y) == exp(x, y + 1.0)
-    {
-      lem_exp_Def(x, y);
-    }
   }
 
 }
