theory/math/LemFunction.dfy
@@ -1,3 +1,4 @@
+include "./Order.dfy"
 include "./TypeR0.dfy"
 
 /******************************************************************************
@@ -6,6 +7,7 @@ include "./TypeR0.dfy"
 
 module LemFunction {
 
+  import opened Order
   import opened TypeR0
 
   ghost function liftD<T>(f:nat->T, default:T) : int->T
@@ -41,36 +43,97 @@ module LemFunction {
   { 
     lem_fun_Ext(x => f1(x)*g1(x), x => f2(x)*g2(x)) by { 
       forall x:A
-         ensures (x => f1(x)*g1(x))(x) == (x => f2(x)*g2(x))(x)
+        ensures (x => f1(x)*g1(x))(x) == (x => f2(x)*g2(x))(x)
       {
       }
     }
   }
 
-  // If f is strictly increasing then f is injective
-  lemma lem_fun_StrictIncrIMPinjective(f:real->real)
+  /******************************************************************************
+    If f:A->A is strictly increasing/decreasing then f is injective
+  ******************************************************************************/
+
+  // General version for any A equipt with Ord<A>
+  lemma lem_fun_StrictIncrIMPinjective<A>(f:A->A, ord:Ord<A>)
+    requires forall x, y :: ord.Lt(x, y) ==> ord.Lt(f(x), f(y))
+    ensures  forall x, y :: f(x) == f(y) ==> x == y
+  {
+    forall x, y | f(x) == f(y)
+      ensures x == y
+    {
+      // By RAA, suppose x != y
+      if x != y {
+        ord.lem_Lt_IfNotEq(x, y); // (x < y) ∨ (y < x) 
+        if ord.Lt(x, y) {
+          assert ord.Lt(f(x), f(y));
+          assert f(x) != f(y) by { ord.lem_Lt_NotEq(f(x), f(y)); }
+          assert false;
+        }
+        else if ord.Lt(y, x) {
+          assert ord.Lt(f(y), f(x));
+          assert f(x) != f(y) by { ord.lem_Lt_NotEq(f(x), f(y)); }
+          assert false;
+        }
+      }
+    }
+  }
+
+  lemma lem_fun_StrictDecrIMPinjective<A>(f:A->A, ord:Ord<A>)
+    requires forall x, y :: ord.Lt(x, y) ==> ord.Gt(f(x), f(y))
+    ensures  forall x, y :: f(x) == f(y) ==> x == y
+  {
+    forall x, y | f(x) == f(y)
+      ensures x == y
+    {
+      // By RAA, suppose x != y
+      if x != y {
+        ord.lem_Lt_IfNotEq(x, y); // (x < y) ∨ (y < x) 
+        if ord.Lt(x, y) {
+          assert ord.Gt(f(x), f(y));
+          assert ord.Lt(f(y), f(x));
+          assert f(x) != f(y) by { ord.lem_Lt_NotEq(f(x), f(y)); }
+          assert false;
+        }
+        else if ord.Lt(y, x) {
+          assert ord.Gt(f(y), f(x));
+          assert ord.Lt(f(x), f(y));
+          assert f(x) != f(y) by { ord.lem_Lt_NotEq(f(x), f(y)); }
+          assert false;
+        }
+      }
+    }
+  }
+
+  // Concrete version for Dafny primitive real type
+  lemma lem_fun_StrictIncrIMPinjectiveReal(f:real->real)
     requires forall x, y :: x < y ==> f(x) < f(y)
     ensures  forall x, y :: f(x) == f(y) ==> x == y
   {
   }
 
-  lemma lem_fun_StrictIncrIMPinjectivePred(f:real->real, p:real->bool)
+  lemma lem_fun_StrictIncrIMPinjectiveRealPred(f:real->real, p:real->bool)
     requires forall x, y :: p(x) && p(y) ==> (x < y ==> f(x) < f(y))
     ensures  forall x, y :: p(x) && p(y) ==> (f(x) == f(y) ==> x == y)
   {
   }    
 
-  // If f is strictly decreasing then f is injective
-  lemma lem_fun_StrictDecrIMPinjective(f:real->real)
+  lemma lem_fun_StrictDecrIMPinjectiveReal(f:real->real)
     requires forall x, y :: x < y ==> f(x) > f(y)
     ensures  forall x, y :: f(x) == f(y) ==> x == y
   {
   }
 
-  lemma lem_fun_StrictDecrIMPinjectivePred(f:real->real, p:real->bool)
+  lemma lem_fun_StrictDecrIMPinjectiveRealPred(f:real->real, p:real->bool)
     requires forall x, y :: p(x) && p(y) ==> (x < y ==> f(x) > f(y))
     ensures  forall x, y :: p(x) && p(y) ==> (f(x) == f(y) ==> x == y)
   {
   } 
+
+  // Concrete version for Dafny primitive nat type
+  lemma lem_fun_StrictIncrIMPinjectiveNat(f:nat->nat)
+    requires forall x, y :: x < y ==> f(x) < f(y)
+    ensures  forall x, y :: f(x) == f(y) ==> x == y
+  {
+  }
 
 }
