theory/math/LemReal.dfy
@@ -1,0 +1,22 @@
+/******************************************************************************
+  Facts about real numbers
+******************************************************************************/
+
+module LemReal {
+
+  // x < y ⟹ ∃ d > 0 : y = x + d
+  lemma lem_real_PosDifference(x:real, y:real)
+    requires x < y
+    ensures  exists d:real {:trigger psPred(x,y,d)} :: d > 0.0 && y == x + d
+  {
+    var d := y - x;
+    assert d > 0.0;
+    assert y == x + d;
+    assert psPred(x,y,d);
+  } 
+
+  ghost predicate psPred(x:real, y:real, d:real) {
+    y == x + d
+  }
+
+}
