theory/math/MaxMin.dfy
@@ -14,13 +14,13 @@ module MaxMin {
     if a < b then a else b
   }
 
-  // n >= 0 ==> max(0,n) = n
+  // n >= 0 ⟹ max(0,n) = n
   lemma lem_max_leftId(n:int)
     requires n >= 0
     ensures max(0, n) == n 
   {}
 
-  // n >= 0 ==> max(0,n) = n
+  // n >= 0 ⟹ max(0,n) = n
   lemma lem_max_rightId(n:int) 
     requires n >= 0
     ensures max(n, 0) == n
