theory/math/Order.dfy
@@ -1,0 +1,112 @@
+/******************************************************************************
+  Order stuff
+******************************************************************************/
+
+module Order {
+
+  // Any type T implementing Ord<T> must provide a predicate Lt(_,_)
+  // and prove it behaves as _<_
+  
+  trait Ord<T(==)> {
+
+    // x < y
+    predicate Lt(x:T, y:T)  
+
+     // x > y
+    predicate Gt(x:T, y:T) { Lt(y, x) }
+
+    // Minimal < properties
+
+    lemma {:axiom} lem_Lt_Irrfl(x:T)
+      ensures !Lt(x, x)
+
+    lemma {:axiom} lem_Lt_Trans(x:T, y:T, z:T)
+      requires Lt(x, y) && Lt(y, z)
+      ensures  Lt(x, z)
+
+    lemma {:axiom} lem_Lt_Antisym(x:T, y:T)
+      requires Lt(x, y)
+      ensures  !Lt(y, x)
+
+    // Relate < to ==
+ 
+    lemma {:axiom} lem_Lt_NotEq(x:T, y:T)
+      requires Lt(x, y)
+      ensures  x != y
+
+    lemma {:axiom} lem_Lt_IfNotEq(x:T, y:T)
+      requires x != y 
+      ensures  Lt(x, y) || Lt(y, x)
+
+  }
+
+  // Implement Ord for nat
+
+  class NatOrd extends Ord<nat> {
+
+    function Lt(x:nat, y:nat): bool {
+      x < y
+    }
+
+    lemma lem_Lt_Irrfl(x:nat)
+      ensures !Lt(x, x)
+    { }
+
+    lemma lem_Lt_Trans(x:nat, y:nat, z:nat)
+      requires Lt(x, y) && Lt(y, z)
+      ensures  Lt(x, z)
+    { }
+
+    lemma lem_Lt_Antisym(x:nat, y:nat)
+      requires Lt(x, y)
+      ensures  !(Lt(y, x))  
+    { }  
+
+    lemma lem_Lt_NotEq(x:nat, y:nat)
+      requires Lt(x, y)
+      ensures  x != y    
+    { }
+
+    lemma lem_Lt_IfNotEq(x:nat, y:nat)
+      requires x != y 
+      ensures  Lt(x, y) || Lt(y, x)   
+    { } 
+
+  }
+
+  // Implement Ord for real
+
+  class RealOrd extends Ord<real> {
+
+    function Lt(x:real, y:real): bool {
+      x < y
+    }
+
+    lemma lem_Lt_Irrfl(x:real)
+      ensures !Lt(x, x)
+    { }
+
+    lemma lem_Lt_Trans(x:real, y:real, z:real)
+      requires Lt(x, y) && Lt(y, z)
+      ensures  Lt(x, z)
+    { }
+
+    lemma lem_Lt_Antisym(x:real, y:real)
+      requires Lt(x, y)
+      ensures  !(Lt(y, x))  
+    { }      
+
+
+    lemma lem_Lt_NotEq(x:real, y:real)
+      requires Lt(x, y)
+      ensures  x != y    
+    { }
+
+    lemma lem_Lt_IfNotEq(x:real, y:real)
+      requires x != y 
+      ensures  Lt(x, y) || Lt(y, x)   
+    { } 
+
+  }  
+
+}
